---
title: Gravitational attraction of a prism
bibliography: references.bib
jupyter: python3
---

```{python}
#| echo: false
from IPython.display import display, Math
from sympy import *
init_printing(use_latex="mathjax", latex_mode="equation")
```

## Problem description

Recall that the vertical component of the gravitational attraction caused by an elongated prismatic body of cross section $S$ is

$$
g_z(x,z) = \frac{\partial}{\partial z}V(x,z) = -2 f \Delta \rho \int\limits_S \frac{(z - z')\, dx' \,dz'}{{(x-x')^2 + (z-z')^2}}.
$$

If the point of observation is at the origin, we obtain

$$
g_z(0,0) = \frac{\partial}{\partial z}V(0,0) = 2 f \Delta \rho \int\limits_S \frac{z\, dx \, dz}{{x^2 + z^2}}.
$$

It can be shown that this surface integral can be equivalently replaced by a line integral taken along the periphery of $S$.

## Line integral

The Stokes theoremÂ states that, for any vector field $\mathbf A = (A_x, 0, A_z)^\top$ there holds

$$
\int\limits_S (\nabla \times \mathbf A) \cdot d\mathbf s = \oint\limits_C \mathbf A \cdot d\mathbf \ell,
$$

where $d\mathbf\ell = \mathbf e_x dx + \mathbf e_z dz$ is the oriented line element tangential to the curve $C$, and $d\mathbf s = dx \,dz \, \mathbf e_y$ the oriented surface element normal to the cross section $S$. It follows by inspection that

$$
\partial_z A_x - \partial_x A_z = 2 f \Delta \rho \frac{z}{x^2 + z^2}
$$

such that, after making the *ansatz* (@zhou2008)

$$
A_x = 0, \qquad A_z = -2 f \Delta\rho \, z \left(\frac{1}{z} \, \tan^{-1}\frac{x}{z}\right) = -2 f \Delta \rho \, \theta
$$

The angle $\theta$ is taken from the positive $x$-axis towards the positive $z$-axis.

@talwani1959 have shown that the vertical component of the gravitational attraction of a two-dimensional prismatic body is, at the origin, equal to

$$
g_z(0, 0) = 2 f \Delta \rho \oint\limits_C z \, d\theta,
$$

i.e., a line integral taken along its periphery.

The following sketch illustrates the situation (taken from the original Talwani paper).

![](https://ruboerner.github.io/images/Talwani-2D.png)

Let $ABCDEF$ be a given polygon with $n$ sides and let $P$ be the point at which the gravitational attraction due to this body has to be computed.

Further, let $z$ be defined positive downwards and let $\theta$ be measured from the positive $x$-axis towards the positive $z$-axis.

Let us evaluate the integral $\oint z\, d\theta$ for the above polygon.

We consider here the contribution from the side $BC$. The remaining sides have to be added to obtain the total gravitational attraction of the complete prism.

At the point $Q$ the line $BC$ meets the $x$-axis at an angle $\phi_i$.

Let $PQ = a_i$. For any arbitrary point $R = R(x,z)$ on the side $BC$ there hold the two equivalent equations

$$
z = x \tan\theta
$$

and

$$
z = (x - a_i) \tan\phi_i.
$$

After eliminating $x$ we obtain an expression for $z = z(\theta)$:

$$
z = \frac{a_i \tan\phi_i \tan\theta}{\tan\phi_i - \tan\theta}
$$

The contribution of the segment $BC$ to the above line integral can now be rewritten as

$$
\int_{BC} z \, d\theta = \int\limits_B^C \frac{a_i \tan\phi_i \tan\theta}{\tan\phi_i - \tan\theta} \, d\theta =: Z_i.
$$

The vertical component of the gravitational attraction is

$$
g_z(0, 0) = 2 f \Delta \rho \sum_{i=1}^n Z_i.
$$

It remains to solve the integral in the expression for $Z_i$. To this end, we use `Sympy`.

## Implementation

```{python}
a, x, z, phi, theta, Z = symbols('a x z phi theta Z', real=True)
Z = solve(
    [tan(theta) * x - z, (x - a) * tan(phi) - z], 
    [x, z], dict=True)
# Z[0][z]
simplify(integrate(Z[0][z], theta))
```
Note that with
$$
\log\left( \frac{1}{\cos^2\theta}\right) = - 2 \log \cos\theta
$$
and after combining the $\log$ terms we obtain the desired integral taken in the limit of integration, i.e., $\theta_i$ and $\theta_{i+1}$
$$
Z_{i} =a_{1} \sin \phi_{i} \cos \phi_{i} \left[ \theta_{i}-\theta_{i+1} +\tan \phi_{i} \log _{s} \frac{\cos \theta_{i}\left(\tan \theta_{i}-\tan \phi_{j}\right)}{\cos \theta_{i+1}\left(\tan \theta_{i+1}-\tan \phi_{i}\right)}\right] 
$$
which is the equation for $Z_i$ given in @talwani1959, p. 50.
---
